theories/examples/finelt/validity.v
@@ -1,0 +1,302 @@
+From Stdlib Require Import Relations List Program
+     ssreflect ssrfun ssrbool.
+From Stdlib Require Import Classes.RelationClasses 
+  Classes.Morphisms Lia Arith.
+
+Set Implicit Arguments.
+Unset Strict Implicit.
+Unset Printing Implicit Defensive.
+
+Require findom.
+Require types.
+Require Import syntax.syntax.
+Require Import syntax.typing.
+
+Import SyntaxNotations.
+Import SubstNotations.
+
+Open Scope syntax_scope.
+
+Module Raw.
+  Include findom.Raw.
+  Include types.
+
+  Lemma le_valid_compatible w u v: 
+    valid w -> le u w -> le v w -> compatible u v.
+  Proof.
+    move=> Vw Lu Lv.
+    eapply comp_down; eauto.
+    eapply compatible_sym.
+    eapply comp_down; eauto.
+    eapply compatible_refl; eauto.
+  Qed.
+End Raw.
+
+Module Valid. 
+  Include findom.Valid.
+
+  Definition wt (u a : Valid.elt) := 
+    Raw.wt (projT1 u) (projT1 a).
+
+  Definition is_bot (v : Valid.elt) : bool := 
+    match projT1 v with 
+    | Raw.bot => true
+    | _ => false
+    end.
+
+  Definition is_abs (v : Valid.elt) : option Valid.finfun := 
+    match v with 
+    | existT _ (Raw.abs e) Vf => Some (existT _ e Vf)
+    | _ => None
+    end.
+
+  Definition is_tpi (v : Valid.elt) : option (Valid.elt * option Valid.finfun).
+    destruct v as [a f].
+    destruct a eqn:Ea.
+    - exact None.
+    - exact None.
+    - exact None.
+    - exact None.
+    - exact None.
+    - apply Some.
+      cbn in f.
+      move:f => /andP [Ve h].
+      split. exists a.
+    match v with 
+    | existT _ (Raw.tpi a nil) => Some (existT _ 
+
+  Definition abs (f : finfun) : elt.
+    exists (Raw.abs (projT1 f)).
+    destruct f as [f Vf]. 
+    eassumption.
+  Defined.
+
+  Definition app (f : finfun) (u : elt) : elt.
+    destruct f as [f Vf].
+    destruct u as [u Vu].
+    destruct (Raw.app f u) eqn:h. 
+    { apply Raw.valid_app in h; eauto.
+      exists e. exact h. } 
+    { assert False.
+      destruct (Raw.valid_app_exists Vf Vu) as [w [Aw Vw]].
+      rewrite Aw in h. done. done. } 
+  Defined.
+
+  Definition graph (f : finfun) : list (elt * elt).
+    destruct f as [f Vf].
+    move: (Raw.valid_fun_subterms Vf) => h.
+    clear Vf.
+    move: h.
+    induction f as [|[u v]f].
+    move=> h. exact nil.
+    cbn.
+    move=> /andP.
+    move=> [/andP h1 h2]. 
+    eapply cons. destruct h1 as [Vu Vv].
+    eapply ((existT _ u Vu),(existT _ v Vv)).
+    eapply IHf; eauto.
+  Defined.
+
+  Lemma le_fun_mono_arg f u1 u2 :
+    le u1 u2 -> le (app f u1) (app f u2).
+  Proof.
+    move=> LE.
+    destruct f as [f Vf].
+    destruct u1 as [u1 Vu1].
+    destruct u2 as [u2 Vu2].
+    unfold le in LE. cbn [projT1] in LE. 
+  Admitted.
+
+End Valid.
+
+Import Valid.
+
+(* Part 1: Finite environments *)
+
+Definition Env n := fin n -> elt.
+
+(* Part 2: EvalRel *)
+
+Notation " a ↦ b " := (Valid.singleton a b) (at level 70).
+Notation " a == b " := (Valid.eqb a b) (at level 70).
+  
+Fixpoint EvalRel {n} (t : Tm n) : Env n -> Valid.elt -> Prop := 
+  match t return Env n -> Valid.elt -> Prop with 
+  | var i => fun ρ b => Valid.le b (ρ i)
+  | tuniv i => fun ρ b =>
+             (* i.e. b == bot \/ b == tuniv i *)
+             Valid.le b (Valid.tuniv i)
+  | tnat => fun ρ b => 
+             (* b == bot \/ b == tnat *)
+             Valid.le b Valid.tnat
+  | zero => fun ρ b => 
+             Valid.le b Valid.zero
+  | succ M => fun ρ b => 
+               if Valid.is_bot b then True else
+                 exists a, Valid.le b (Valid.succ a) /\ EvalRel M ρ a
+  | tpi A B => fun ρ b => 
+        if is_bot b then True
+        else match is_tpi b with 
+              | Some (a, ff) =>
+                  exists i a', wt a (tuniv i) /\ EvalRel A ρ a /\
+                    match ff with 
+                    | Some g =>         
+                        forall u v, In (u,v) (graph g) -> 
+                               exists x, le x u /\ wt x a /\
+                                      EvalRel B (x .: ρ) v
+                    | None => True 
+                    end
+              | None => False
+             end
+
+         match projT1 b with 
+         | Raw.bot => True
+         | Raw.tpi a f =>              
+             (exists a', EvalRel A ρ a' /\
+                      forall u v, Raw.app f (projT1 u) = Some (projT1 v) -> 
+                             exists (x : Valid.elt), 
+                               Valid.le x u 
+                               /\ wt (projT1 x) (projT1 a')
+                               /\ EvalRel B (x .: ρ) v)
+         | _ => False
+         end
+  | app M N => fun ρ b => 
+         if Valid.is_bot b then True else 
+            exists a, EvalRel M ρ (a ↦ b) /\ EvalRel N ρ a 
+  | abs A M => fun ρ b => 
+         match b with 
+         | existT _ Raw.bot _ => True
+         | existT _ (Raw.abs rg) Vg =>
+             exists i a, Valid.wt a (Valid.tuniv i) /\ EvalRel A ρ a
+                    /\ forall u v, In (u,v) (Valid.graph (existT _ rg Vg)) -> 
+                             exists x, Valid.le x u 
+                                  /\ Valid.wt x a
+                                  /\ EvalRel M (x .: ρ) v
+         | _ => False 
+         end
+  | nrec T M0 M1 => fun ρ b =>
+         if Valid.is_bot b then True else False                  
+  end.
+
+
+(* monotonicity *)
+Definition LeEnv {n} (ρ1 ρ2 : Env n) := 
+  forall x, Valid.le (ρ1 x) (ρ2 x).
+
+Lemma EvalRel_mono_env {n} (M : Tm n) (ρ ρ' : Env n) u :
+  EvalRel M ρ u -> LeEnv ρ ρ' -> EvalRel M ρ' u.
+Proof.
+  dependent induction M.
+  all: cbn [EvalRel].
+  all: eauto.
+  all: move=> h1 h2. 
+  - (* M = x *)
+    specialize (h2 f).
+    eapply Valid.le_trans; eauto.
+  - (* M = Abs M1 M2,  *)
+    destruct u as [u Vu]. 
+    destruct u eqn:Eq; try done.
+    move: h1 => [i [a [WT [ER f]]]].
+    exists i ,a. repeat split; eauto.
+    move=> u1 v1 h3. 
+    specialize (f u1 v1 h3).
+    destruct f as [x [Lex [WT2 EM2]]].
+    exists x. repeat split; eauto.
+    eapply IHM2; eauto.
+    unfold LeEnv. move=> [y|]. cbn. eauto.
+    cbn. eapply Valid.le_refl.
+  - (* M = app M1 M2 *)
+    destruct (Valid.is_bot u); try done.
+    destruct h1 as [a [E1 E2]].
+    exists a. split; eauto.
+  - (* M = succ M *)
+    destruct (Valid.is_bot u); try done.
+    destruct h1 as [a [EQ1 E]].
+    exists a. split; eauto.
+  - (* M = tpi M1 M2 *)
+    destruct (projT1 u); try done.
+    destruct h1 as [a [E1 h3]].
+    exists a. split; eauto.
+    intros u1 v1 APP.
+    specialize (h3 u1 v1 APP).
+    destruct h3 as [x [Lx [WT E2]]].
+    exists x. repeat split; eauto.
+    eapply IHM2; eauto.
+    unfold LeEnv. move=> [y|]. cbn. eauto.
+    cbn. eapply Valid.le_refl.
+Qed.    
+
+
+
+(* Lam-edgewise *)
+Lemma lam_edgewise {n} {A : Tm n} {M ρ g} : 
+  EvalRel (abs A M) ρ (Valid.abs g) -> 
+  exists a, EvalRel A ρ a 
+       /\ forall u v, In (u,v) (Valid.graph g) -> 
+         exists x, wt (projT1 x) (projT1 a) /\ EvalRel M (x .: ρ) v.
+Proof.
+  move=> E1.
+  destruct g as [g Vg].
+  cbn [EvalRel projT1 Valid.abs] in E1.
+  destruct E1 as [i [a [WT [EA body]]]].
+  exists a. split; eauto.
+  intros u v ein.
+  destruct (Raw.valid_app_exists Vg (projT2 u)) as [rw [EQ Vw]].
+  specialize (body u v ein).
+  remember (existT (fun x => Raw.valid x) rw Vw) as w.
+  destruct body as [x [Lex [WT2 ER2]]].
+  exists x. split; eauto.
+Qed.
+
+Lemma EvalRel_bot {n} (M : Tm n) (ρ : Env n) : 
+  EvalRel M ρ Valid.bot.
+Proof.
+  destruct M eqn:EQ; cbn; try done.
+  (* var *) rewrite Valid.le_bot; eauto.
+Qed.
+
+
+Lemma EvalRel_compatible {n} (M : Tm n) :
+  forall (ρ : Env n) (a b : Valid.elt),
+  EvalRel M ρ a -> EvalRel M ρ b -> Raw.compatible (projT1 a) (projT1 b).
+Proof.
+  induction M.
+  all: cbn [EvalRel].
+  all: move=> ρ a b.
+  - (* var *) 
+    move=> /andP h1 /andP h2. 
+    move: h1 => [C1 L1]. move: h2 => [C2 L2].
+    destruct (ρ f) as [rf Vf]. cbn in *.
+    eapply Raw.le_valid_compatible; eauto.
+  - (* abs M1 M2 *)
+    destruct a as [a Va]. destruct b as [b Vb].
+    move=> h1 h2.
+    destruct a; try done;
+    destruct b; try done.
+    destruct h1 as [i1 [a1 [WT1 [E1 F1]]]].
+    destruct h2 as [i2 [a2 [WT2 [E2 F2]]]].
+    cbn [projT1 Raw.compatible].
+    apply /forallb_forall.
+    move=> [ui vi] Ini.
+    apply /forallb_forall. 
+    move=> [uj vj] Inj.
+    apply /implyP. move=> h1.
+    move: (Raw.valid_fun_subterms Va) => /forallb_forall Vs1.
+    specialize (Vs1 _ Ini). move: Vs1 => /andP [Vui Vvi].
+    move: (Raw.valid_fun_subterms Vb) => /forallb_forall Vs2.
+
+    have: valid ui.
+(*
+-- Val G M A u a : term M has type A, with realizer u at code a, in context G
+ Val : {n : Nat} -> Ctx n -> Expr n -> Expr n -> FinEl -> FinEl -> Set
+*)
+
+Fixpoint Val {n: nat} (Γ : Ctx n) ( M : Tm n) (A : Tm n)  (u : Raw.elt) (a : Raw.elt) : Prop.
+destruct a eqn:Ea.
+- exact True.  
+- destruct u eqn:Eu.
+  + exact True.
+  + exact False.
+  + exact False.
+  + exact True.
+  + destruct M eqn:EM.
