theories/examples/syntax/typing.v
@@ -1,0 +1,421 @@
+Require Import ssreflect.
+
+Require Import syntax.
+Require Export fintype.
+Require Export fin_util.
+
+Require Export Logic.FunctionalExtensionality.
+Require Import Stdlib.Program.Equality.
+
+Lemma ext_fin {n A}{f g: fin n -> A} : 
+  (forall x, f x = g x) -> f = g.
+eapply functional_extensionality.
+Qed.
+
+Import ScopedNotations.
+Import SubstNotations.
+
+Disable Notation "'__Tm'" (all).
+
+(** Define a notation scope specific to this language. *)
+Declare Scope syntax_scope.
+
+Module SyntaxNotations.
+Export ScopedNotations.
+Notation "⇑" := (up_Tm_Tm) : syntax_scope.
+Notation "⇑ σ" := (var var_zero .: σ >> ren_Tm ↑) 
+                    (only printing, at level 0) : syntax_scope.
+End SyntaxNotations.
+Import SyntaxNotations.
+
+Create HintDb syntax.
+Open Scope syntax_scope.
+
+
+Inductive Ctx : nat -> Type := 
+| ctx_empty    : Ctx 0
+| ctx_extend n : Ctx n -> Tm n -> Ctx (S n).
+
+Notation "Γ ++ A" := (ctx_extend _ Γ A) : syntax_scope.
+
+Fixpoint lookup {n} (x : fin n) : Ctx n -> Tm n.
+  destruct n; cbn in x. done.
+  destruct x as [p|]. 
+  - move=> tl.
+    inversion tl. exact (lookup _ p X)⟨↑⟩.
+  - move=> tl.
+    inversion tl. exact (X0⟨↑⟩).
+Defined.
+
+
+(*
+Definition Ctx n := fin n -> Tm n.
+
+Definition Ctx_app {n} : Ctx n -> Tm n -> Ctx (S n) := 
+  fun Γ A => ( A⟨↑⟩ .: (Γ >> ⟨↑⟩)).
+
+Notation "Γ ++ A" := (Ctx_app Γ A).
+*)
+
+
+(* for nrec *)
+Definition rho {n} : fin (S n) -> Tm (S n) := 
+   (succ (var var_zero) .: var >> ⟨↑⟩).
+
+Inductive typing : forall {n} (Γ : Ctx n), Tm n -> Tm n -> Prop := 
+  | t_var n (Γ : Ctx n) x : 
+    ctx Γ ->
+    typing Γ (var x) (lookup x Γ)
+  | t_conv n (Γ : Ctx n) M A B i : 
+    typing Γ M A -> 
+    conv Γ A B (tuniv i) -> 
+    typing Γ M B
+  | t_abs n (Γ : Ctx n) A B N i : 
+    typing Γ A (tuniv i) ->
+    typing (Γ ++ A) B (tuniv i) -> 
+    typing (Γ ++ A) N B ->
+    typing Γ (abs A N) (tpi A B)
+  | t_app n (Γ : Ctx n) A B N M i : 
+    typing Γ A (tuniv i) -> 
+    typing (Γ ++ A) B (tuniv i) -> 
+    typing Γ N (tpi A B) ->
+    typing Γ M A -> 
+    typing Γ (app N M) B[M..]
+  (* natural numbers *)
+  | t_nat n (Γ : Ctx n) : 
+    typing Γ tnat (tuniv 0)
+  | t_zero n (Γ : Ctx n) : 
+    typing Γ zero tnat 
+  | t_succ n (Γ : Ctx n) M : 
+    typing Γ M tnat ->
+    typing Γ (succ M) tnat 
+  | t_nrec n (Γ : Ctx n) (T U : Tm (S n)) M0 M1 i :
+    typing (Γ ++ tnat) T (tuniv i) ->
+    typing Γ M0 (T[zero..]) ->
+    U = T[rho] ->
+    typing Γ M1 (tpi tnat (tpi T U⟨↑⟩ )) ->       
+    typing Γ (nrec T M0 M1) (tpi tnat T)
+  (* universes *)
+  | t_tpi n (Γ : Ctx n) A B i : 
+    typing Γ A (tuniv i) ->
+    typing (Γ ++ A) B (tuniv i) -> 
+    typing Γ (tpi A B) (tuniv i)
+  | t_cum n (Γ : Ctx n) A i j : 
+    typing Γ A (tuniv i) -> (i < j)%nat -> 
+    typing Γ A (tuniv j)
+  | t_univ n (Γ : Ctx n) i j : 
+    (i < j)%nat ->
+    typing Γ (tuniv i) (tuniv j)
+with conv :forall {n} (Γ : Ctx n), Tm n -> Tm n -> Tm n -> Prop := 
+  | c_conv n (Γ : Ctx n) M N A B i : 
+    conv Γ M N A -> 
+    conv Γ A B (tuniv i) ->
+    conv Γ M N B
+  | c_refl n (Γ : Ctx n) M A : 
+    typing Γ M A ->
+    conv Γ M M A 
+  | c_trans n (Γ : Ctx n) M N P A  : 
+    conv Γ M N A -> 
+    conv Γ N P A -> 
+    conv Γ M P A
+  | c_app1 n (Γ : Ctx n) A B N N' M i : 
+    typing Γ A (tuniv i) -> 
+    typing (Γ ++ A) B (tuniv i) -> 
+    conv Γ N N' (tpi A B) ->
+    typing Γ M A ->
+    conv Γ (app N M) (app N' M) B[M..]
+  | c_app2 n (Γ : Ctx n) A B N M M' i  :          
+    typing Γ A (tuniv i) -> 
+    typing (Γ ++ A) B (tuniv i) -> 
+    typing Γ N (tpi A B) ->
+    conv Γ M M' A ->
+    conv Γ (app N M) (app N M') B[M..]
+  | c_beta n (Γ : Ctx n) A B M N i :
+    typing Γ A (tuniv i) -> 
+    typing (Γ ++ A) B (tuniv i) -> 
+    typing (Γ ++ A) N B -> 
+    typing Γ M A ->
+    conv Γ (app (abs A N) M) N[M..] B[M..]
+  | c_eta n (Γ : Ctx n) A B N N' i :
+    typing Γ A (tuniv i) -> 
+    typing (Γ ++ A) B (tuniv i) -> 
+    typing Γ N (tpi A B) ->     
+    typing Γ N' (tpi A B) ->     
+    conv (Γ ++ A) (app N⟨↑⟩ (var var_zero))
+      (app N'⟨↑⟩ (var var_zero)) A⟨↑⟩ ->
+    conv Γ N N' (tpi A B)
+  (* natural numbers: TODO add typing hyps *)
+  | c_nrec_Z n (Γ : Ctx n) M0 M1 (T : Tm (S n)) i : 
+    typing  (Γ ++ tnat) T (tuniv i) ->
+    typing Γ M0 (T[zero..]) ->
+    typing Γ M1 (tpi tnat (tpi T T[rho]⟨↑⟩ )) ->   
+    conv Γ (app (nrec T M0 M1) zero) M0 T[zero..]
+  | c_nrec_S n (Γ : Ctx n) T M0 M1 n i : 
+    typing (Γ ++ tnat) T (tuniv i) ->
+    typing Γ M0 (T[zero..]) ->
+    typing Γ M1 (tpi tnat (tpi T T[rho]⟨↑⟩ )) ->    
+    conv Γ (app (nrec T M0 M1) (succ n)) 
+      (app (app M1 n) (app (nrec T M0 M1) n)) T[(succ n)..]
+  | c_tuniv n (Γ : Ctx n) M N i j : 
+    conv Γ M N (tuniv i) -> (i < j)%nat ->
+    conv Γ M N (tuniv j)
+  | c_tpi n (Γ : Ctx n) A0 A1 B0 B1 i :
+    conv Γ A0 A1 (tuniv i) -> 
+    conv (Γ ++ A0) B0 B1 (tuniv i) -> 
+    conv Γ (tpi A0 B0) (tpi A1 B1) (tuniv i)
+with ctx : forall {n}, Ctx n -> Prop :=
+  | c_empty : ctx ctx_empty
+  | c_cons n (Γ : Ctx n) A i : ctx Γ -> 
+     typing Γ A (tuniv i) -> 
+     ctx (Γ ++ A).
+
+
+(*
+Lemma ctx_extend {n} {Γ:Ctx n}{A:Tm n} :
+  ctx Γ -> type Γ A -> ctx (Γ ++ A).
+Proof. move=> [ih] hT. constructor.
+       auto_case. 
+*)
+
+(** This version of t_var is easier to work with sometimes
+    as it doesn't require the type to already be in the form 
+    Γ x. *)
+Definition t_var' {n} (Γ : Ctx n) x τ : 
+  lookup x Γ = τ -> ctx Γ -> typing Γ (var x) τ.
+intros <-. eapply t_var. Qed.
+Definition t_app' {n} (Γ : Ctx n) (A : Tm n) 
+  (B : Tm (S n)) (N M : Tm n) (C:Tm n) i :
+       typing Γ A (tuniv i) ->
+            typing (Γ ++ A) B (tuniv i) -> typing Γ N (tpi A B) 
+       -> typing Γ M A 
+       -> B[M..] = C
+       -> typing Γ (app N M) C.
+intros. subst. eapply t_app; eauto. Qed. 
+Definition t_univ' {n} (Γ : Ctx n) A (i j : nat):
+  i < j -> tuniv j = A -> 
+  typing Γ (tuniv i) A.
+intros h1 <-. eapply t_univ; eauto. Qed.
+Definition t_cum' {n} (Γ : Ctx n) A i j B : 
+    typing Γ A (tuniv i) -> (i < j)%nat -> 
+    tuniv j = B ->
+    typing Γ A B.
+Proof. intros; subst; eauto using t_cum. Qed.
+
+#[export] Hint Resolve t_var'  t_univ': syntax.
+
+#[export] Hint Constructors typing conv : syntax.
+
+
+Module Notations.
+Notation "Γ |-e a ∈ A" := (typing Γ a A) (at level 70) : syntax_scope.
+Notation "Γ |-e a ≡ b ∈ A" := (conv Γ a b A) (at level 70) : syntax_scope.
+End Notations.
+
+Open Scope syntax_scope.
+Import Notations.
+
+(** * Renaming and substitution properties *)
+
+(* == RenTypes *)
+(*
+Definition typing_renaming {n} (Δ : fin n -> Tm n) 
+  {m} (δ : fin m -> fin n)
+  (Γ : fin m -> Tm m) : Prop := 
+  forall i, Δ (δ i) = (Γ i)⟨δ⟩.
+*)
+Definition typing_renaming {n} (Δ : Ctx n) 
+  {m} (δ : fin m -> fin n)
+  (Γ : Ctx m) : Prop := 
+  forall i, lookup (δ i) Δ  = (lookup i Γ)⟨δ⟩.
+
+
+(** The identity renaming preserves the context *)
+Lemma typing_renaming_id {n} (Δ : Ctx n) :
+  typing_renaming Δ id Δ.
+Proof. unfold typing_renaming. intros x. asimpl. done. Qed.
+
+(** shift extends the context *)
+Lemma typing_renaming_shift {n} (Γ : Ctx n) (τ : Tm n) :
+    typing_renaming (Γ ++ τ) shift Γ.
+Proof.
+  unfold typing_renaming. intros x. asimpl. fsimpl. done. Qed.
+
+(** Lift a renaming to a new scope *)
+Lemma typing_renaming_lift {n} (Δ : Ctx n) 
+  {m} (Γ : Ctx m) (δ : fin m -> fin n) (τ : Tm m) :
+  typing_renaming Δ δ Γ ->
+  typing_renaming (Δ ++ τ⟨δ⟩) (up_ren δ) (Γ ++ τ).
+Proof. intro h. unfold typing_renaming in *.
+       auto_case; asimpl; try done.
+       unfold ">>". rewrite h.
+         asimpl. done.
+Qed.
+
+Create HintDb renaming.
+#[export] Hint Resolve typing_renaming_lift 
+  typing_renaming_id typing_renaming_shift : renaming.
+
+
+Fixpoint renaming_typing {n} (Γ : Ctx n) a A {m} (Δ:Ctx m) δ : 
+  Γ |-e a ∈ A -> typing_renaming Δ δ Γ -> ctx Δ -> Δ |-e a⟨δ⟩ ∈ A⟨δ⟩
+with renaming_conv {n} (Γ : Ctx n) a b A {m} (Δ:Ctx m) δ : 
+  Γ |-e a ≡ b ∈ A -> typing_renaming Δ δ Γ ->  ctx Δ -> Δ |-e a⟨δ⟩ ≡ b⟨δ⟩ ∈ A⟨δ⟩
+(*
+with renaming_type {n} (Γ : Ctx n) A {m} (Δ:Ctx m) δ : 
+  Γ |-τ A -> typing_renaming Δ δ Γ ->  ctx Δ -> Δ |-τ A⟨δ⟩
+with renaming_type_conv {n} (Γ : Ctx n) A B {m} (Δ:Ctx m) δ : 
+  Γ |-τ A ≡ B -> typing_renaming Δ δ Γ ->  ctx Δ -> Δ |-τ A⟨δ⟩ ≡ B⟨δ⟩
+with ctx_extend {n} {Γ:Ctx n}{A:Tm n} :
+  ctx Γ -> type Γ A -> ctx (Γ ++ A)
+*).
+Proof. 
+  have renaming_typing': 
+    forall n (Γ : Ctx n) a A {m} (Δ:Ctx m) δ B,
+      Γ |-e a ∈ A -> typing_renaming Δ δ Γ ->  ctx Δ ->
+         B = A⟨δ⟩ ->
+         Δ |-e a⟨δ⟩ ∈ B.
+  { admit. }
+  have renaming_conv' :
+    forall n (Γ : Ctx n) a b A {m} (Δ:Ctx m) δ B,
+      Γ |-e a ≡ b ∈ A -> typing_renaming Δ δ Γ ->  ctx Δ ->
+         B = A⟨δ⟩ ->
+         Δ |-e a⟨δ⟩ ≡ b⟨δ⟩ ∈ B.
+  { admit. } 
+  (* typing *)
+  - intros h tR wtΔ. 
+    dependent destruction h; subst.
+    all: asimpl.
+    all: try solve [econstructor; eauto with renaming; cbn].
+    + (* var case *)
+      eapply t_var'; eauto.
+    + (* conv *) 
+      econstructor; eauto with renaming.
+      eapply renaming_conv'; eauto.
+      cbn; eauto.
+    + (* abs *)
+      have EC: ctx (Δ ++ A ⟨δ⟩).
+      { eapply c_cons; eauto with renaming.
+        eapply renaming_typing in h1; eauto with renaming. } 
+      eapply t_abs; eauto with renaming.
+      eapply renaming_typing' in h1; eauto with renaming.
+      cbn; eauto.
+      eapply renaming_typing in h2; eauto with renaming.
+    + (* app *) 
+      have EC: ctx (Δ ++ A ⟨δ⟩).
+      { eapply c_cons; eauto with renaming.
+        eapply renaming_typing in h1; eauto with renaming. } 
+      eapply t_app' with (B:=B⟨up_ren δ⟩); eauto with renaming. 
+      eapply renaming_typing' in h1; eauto with renaming.
+      cbn; eauto.
+      eapply renaming_typing' in h2; eauto with renaming.
+      eapply renaming_typing' in h3; eauto with renaming.
+      asimpl.
+      auto.
+    + (* nrec *)
+      have EC: ctx (Δ ++ tnat).
+      { eapply c_cons; eauto with renaming.
+        eapply t_nat; eauto. } 
+      eapply t_nrec; eauto with renaming. 
+      eapply renaming_typing' in h1; eauto with renaming.
+      eapply typing_renaming_lift with (τ:=tnat) in tR; eauto.
+      reflexivity.
+      eapply renaming_typing' in h2; eauto. asimpl. eauto.
+      eapply renaming_typing' in h3; eauto with renaming.
+      asimpl. 
+      f_equal. f_equal. 
+      admit. (* ugh! *)
+    + (* tpi *)
+      eapply t_tpi; eauto with renaming.
+      eapply renaming_typing'; eauto with renaming.
+      eapply c_cons; eauto.
+      eapply renaming_typing'; eauto with renaming.
+      reflexivity.
+    + (* tcum *)
+      eapply t_cum'; eauto.
+      eapply renaming_typing'; eauto.
+  (* conv *)
+  - intros h tR tΔ.
+    dependent destruction h; subst.
+    all: asimpl.
+    all: try solve [econstructor; eauto with renaming].
+    + admit.
+    + (* c_app1 *)
+      admit.
+    + (* c_app2 *)
+      admit.
+    + (* c_beta *)
+      admit.
+    + (* c_eta *)
+      admit.
+    + (* c_nrec_zero *)
+      admit.
+    + (* c_rec_succ *)
+      admit.
+    + (* c_cum *)
+      admit.
+    + (* c_tpi *)
+      admit.
+Admitted.    
+
+(** Substution lemmas *)
+
+Definition typing_subst {n} (Δ : Ctx n) {m} (σ : fin m -> Tm n)
+  (Γ : Ctx m) : Prop := 
+  forall x, (Δ |-e (σ x) ∈ (lookup x Γ)[σ]).
+
+Lemma typing_subst_null {n} (Δ : Ctx n) :
+  typing_subst Δ null ctx_empty.
+Proof. unfold typing_subst. auto_case. Qed.
+
+Lemma typing_subst_id {n} (Δ : Ctx n) :
+  ctx Δ -> typing_subst Δ var Δ.
+Proof. move=>h. 
+       unfold typing_subst. intro x. asimpl. econstructor; eauto. 
+       Qed.
+
+(*
+Lemma typing_subst_cons {n} (Δ : Ctx n) {m} (σ : fin m -> Tm n)
+  (Γ : Ctx m) e τ : 
+ Δ |-e e ∈ τ -> typing_subst Δ σ Γ ->
+ typing_subst Δ (e .: σ) (Γ ++ τ).
+Proof. intros. unfold typing_subst in *. intros [y|]; asimpl; eauto. Qed.
+*)
+Lemma typing_subst_lift {n} (Δ : Ctx n) {m} (σ : fin m -> Tm n)
+  (Γ : Ctx m) τ : 
+  ctx (Δ ++ τ[σ]) ->
+  typing_subst Δ σ Γ -> typing_subst (Δ ++ τ[σ]) (⇑ σ) (Γ ++ τ).
+Proof.
+  unfold typing_subst in *.
+  intros EC h.
+  intro x. destruct x.
+  + specialize (h f).
+    cbn.
+    eapply renaming_typing with (Δ := Δ ++ τ[σ])in h;
+      eauto with renaming.
+    asimpl in h. done.
+  +  cbn. eapply t_var'; eauto.
+     cbn. asimpl. eauto.
+Qed.
+
+(** Add the substitution lemmas as hints *)
+#[export] Hint Resolve typing_subst_lift (* typing_subst_cons *)
+             typing_subst_id typing_subst_null : rec.
+
+Fixpoint
+  substitution_tm {n} (Γ : Ctx n) a A {m} (Δ:Ctx m) σ : 
+  Γ |-e a ∈ A -> typing_subst Δ σ Γ -> ctx Δ -> Δ |-e a[σ] ∈ A[σ]
+with 
+ substitution_conv {n} (Γ : Ctx n) a b A {m} (Δ:Ctx m) σ : 
+  Γ |-e a ≡ b ∈ A -> typing_subst Δ σ Γ -> ctx Δ -> Δ |-e a[σ] ≡ b[σ] ∈ A[σ]
+.
+Proof.
+  all: intros h tS tΔ.
+  - dependent destruction h; subst.
+    all: cbn; asimpl.
+    all: try solve [econstructor; eauto with syntax].
+    + unfold typing_subst in tS. eauto.
+    + admit.
+Admitted.
+
+
+
